ems/SimModSemFacts.v
@@ -25,135 +25,289 @@ Import TAC.
 Section ADEQUACY.
   (* Context {CONF: EMSConfig}. *)
 
-  Lemma sim_ctx_mod
-    ctx md1 md2
-    (SIM: ModPair.sim md1 md2)
-
-  :
-    ModPair.sim (Mod.add md1 ctx) (Mod.add md2 ctx)
-  .
-  Proof.
-    inv SIM.
-    econs; et.
-    (* - i. ss. hexploit (sim_modsem sk); et. *)
-    - i. ss. hexploit (sim_modsem sk); et.
-
-      2: { ii. des. apply sim_ctx; et. }
-      unfold Sk.incl, Sk.add in *. i. ss.
-      apply SKINCL.
-      rewrite in_app_iff. et.
-    - r. ss. unfold Sk.add. ss.
-      rewrite sim_sk. et.
-  Qed.
-
-  Lemma adequacy_mod
-          md_src md_tgt
+  Lemma adequacy_modsem
+          ms_src ms_tgt (P Q : Prop)
           (CONF: EMSConfig)
-          (SIM: ModPair.sim md_src md_tgt)
+          (WF: Q -> P)
+          (SIM: ModSemPair.sim ms_src ms_tgt)
     :
-    <<REF: Beh.of_program (Mod.compile md_tgt) <1= Beh.of_program (Mod.compile md_src) >>
-    .
+    <<REF: Beh.of_program (@ModSem.compile ms_tgt CONF (Some P)) <1= Beh.of_program (@ModSem.compile ms_src CONF (Some Q)) >>.
   Proof.
-    ii. unfold Mod.compile in *.
-    destruct (classic (ModSem.wf (Mod.enclose (md_src)) /\ Sk.wf (Mod.sk md_src))).
-    2: { eapply ModSem.initial_itr_not_wf. ss. }
-    ss. des. 
-    pose (sk_tgt := (Mod.sk (md_tgt))).
-    pose (sk_src := (Mod.sk (md_src))).
-    assert (SKEQ: sk_src = sk_tgt).
-    { unfold sk_tgt, sk_src. inv SIM. et. }
-    unfold Mod.enclose in *. fold sk_src in H. inv H.
-    inv SIM. hexploit (sim_modsem (Sk.canon sk_tgt)).
-    { etrans; [|eapply Sk.sort_incl]. ss. }
-    { ss. rewrite sim_sk in H0.
-      clear - H0.
-      unfold Sk.wf in *. ss.
-      eapply Permutation.Permutation_NoDup; [|et].
-      eapply Permutation.Permutation_map.
-      eapply Sk.SkSort.sort_permutation. }
-    i. des.
-    inv H. ss.
+    red. inv SIM. eapply adequacy_local_aux with (wf:=wf) (le:=le); et.
+    i. destruct (alist_find fn (ModSem.fnsems ms_src)) eqn:SRC; destruct (alist_find fn (ModSem.fnsems ms_tgt)) eqn:TGT; et; cycle 1.
+    - eapply alist_find_some in SRC.
+      eapply Forall2_In_l with (a:= (fn, i)) in sim_fnsems; et.
+      inv sim_fnsems. des.
+      destruct x. inv H0. unfold "@@1" in H1. ss. clarify.
+      apply alist_find_none with (v:=i0) in TGT. clarify. 
+    - right. esplits; et. clear -sim_fnsems SRC TGT.
+      revert fn i i0 SRC TGT.
+      induction sim_fnsems; i; ss.
+      des_ifs_safe. inv H. unfold "@@1" in H0. ss. clarify.
+      des_ifs. eapply IHsim_fnsems; et.
+  Qed.
 
-    assert (WFTGT: Mod.wf md_tgt).
-    { rr. unfold Mod.enclose. ss. fold sk_tgt. 
-      rewrite SKEQ in *. split; auto.
-      2: { rewrite <-SKEQ. unfold sk_src. et. }
-      econs.
-      match goal with
-        | H: NoDup ?l0 |- NoDup ?l1 => replace l1 with l0
-      end; auto.
-      eapply Forall2_eq. eapply Forall2_apply_Forall2; et.
-      i. destruct a, b. inv H. ss.
-    }
+  Context `{Sk.ld}.
 
-    eapply adequacy_local_aux in PR; et.
-    - i. esplits.
-      pose (ms_src := Mod.get_modsem md_src (Sk.sort (Mod.sk md_src))).
-      pose (ms_tgt := Mod.get_modsem md_tgt (Sk.sort (Mod.sk md_tgt))).
-      fold ms_src ms_tgt.
-      rewrite <- SKEQ in sim_fnsems at 1.
-      unfold sk_src, sk_tgt in sim_fnsems.
-      fold ms_src ms_tgt in sim_fnsems.
-      hexploit sim_fnsems. i.
-
-      destruct (alist_find fn (ModSem.fnsems ms_src)) eqn:SRC; destruct (alist_find fn (ModSem.fnsems ms_tgt)) eqn:TGT; et.
-      2: {
-        right.
-        eapply alist_find_some in SRC.
-        rewrite <- sim_sk in sim_fnsems.
-        (* eapply alist_find_none in TGT. *)
-        eapply Forall2_In_l with (a:= (fn, i)) in sim_fnsems; et.
-        inv sim_fnsems. inv H1.
-        inv H3. inv H1.
-        destruct x. ss. clarify.
-        apply alist_find_none with (v:=i0) in TGT. clarify. 
-      }
-      right. esplits; et.
-
-      hexploit SRC. hexploit TGT. i.
-      apply alist_find_some in H1, H2.
-
-      rewrite <- sim_sk in sim_fnsems.
-
-      eapply Forall2_In_l with (a:=(fn, i)) in sim_fnsems; et.
-      eapply Forall2_In_r with (b:=(fn, i0)) in H; et.
-      inv sim_fnsems. inv H.
-      destruct x, x1.
-      inv H3. inv H5. inv H3. ss.
-      inv H4. inv H7. inv H4. ss. clarify.
-      unfold "@@2" in H5, H6. ss.
-      (* apply NoDup_map_inv in wf_fnsems. *)
-      unfold sk_src in wf_fnsems.
-      fold ms_src in wf_fnsems.
-      rewrite <- sim_sk in H3.
-      eapply alist_find_some_iff  with (k:=s) (v:=i2) in wf_fnsems; et.
-      rewrite SRC in wf_fnsems. clarify. apply H5.
-    (* - inv sim_initial. econs. econs.
-      2: { fold sk_src sk_tgt. rewrite SKEQ. apply H. }
-      instantiate (1:= x). refl. *)
-
-    Qed.
-
-
-  Theorem adequacy_local_strong md_src md_tgt
-          (SIM: ModPair.sim md_src md_tgt)
+  Theorem adequacy_local_strong_l mds_src mds_tgt
+          (SIM: forall sk, ModLPair.sim mds_src mds_tgt sk)
     :
-    <<CR: (refines_strong md_tgt md_src)>>
+      <<CR: (refines_strong (Mod.add_list mds_tgt) (Mod.add_list mds_src))>>
   .
   Proof.
+  (*   ii. unfold Mod.compile, Mod.enclose in *. *)
+  (*   set (Mod.wf _) as wf_src. set (Mod.wf _) as wf_tgt in PR. *)
+  (*   set (Mod.sk _) as sk_src. set (Mod.sk _) as sk_tgt in PR. *)
+  (*   specialize (SIM (Sk.canon sk_tgt)). inv SIM. *)
+  (*   destruct (classic wf_src); cycle 1. *)
+  (*   { eapply ModSem.compile_not_wf; et. } *)
+  (*   ss. rename H0 into SKWF. *)
+  (*   assert (SKEQ: sk_src = sk_tgt). *)
+  (*   { unfold sk_src, sk_tgt. ss. f_equal. clear -sim_sk. *)
+  (*     ginduction mds_src; i. *)
+  (*     - inv sim_sk. destruct mds_tgt; clarify. *)
+  (*     - destruct mds_tgt; inv sim_sk. ss. destruct mds_src; ss. *)
+  (*       + destruct mds_tgt; inv H5. et. *)
+  (*       + destruct mds_tgt; inv H5. ss. f_equal; et. specialize (IHmds_src (t1 :: mds_tgt)). *)
+  (*         ss. apply IHmds_src. econs; et. } *)
+  (*   hexploit sim_modsem; et. *)
+  (*   { clear. unfold sk_tgt. clear sk_tgt. *)
+  (*     ss. set (Mod.sk ctx) as sk_ctx. *)
+  (*     clearbody sk_ctx. clear ctx. *)
+  (*     ginduction mds_tgt; i; ss. *)
+  (*     econs; cycle 1. *)
+  (*     { destruct mds_tgt; ss. specialize (IHmds_tgt (Sk.add (Mod.sk a) sk_ctx)). *)
+  (*       eapply Forall_impl; [|et]. unfold flip. i. etrans; et. *)
+  (*       etrans. apply Sk.le_canon_rev. etrans; [|apply Sk.le_canon]. *)
+  (*       rewrite Sk.add_assoc. Print Sk.ld. apply IHmds_tgt. } *)
+  (*     ss. etrans; [|apply Sk.le_canon]. etrans; [|apply Sk.le_add_l]. *)
+  (*     apply Sk.le_add_r. } *)
+  (*   { inv SKWF. rewrite <- SKEQ. apply Sk.wf_canon; et. } *)
+  (*   intro SIM. *)
+  (*   destruct wf_tgt; cycle 1. *)
+  (*   { exfalso. apply n. unfold Mod.wf in *. ss. *)
+  (*     fold sk_tgt. rewrite <- SKEQ. des. split; et. ss. *)
+  (*     inv WF. econs; ss; unfold ModSem.add_fnsems in *; rewrite map_app in *. *)
+  (*     i. set (List.map fst _) as ndom_src at 2. *)
+  (*     set (List.map fst _) as ndom_tgt in wf_fnsems at 2. *)
+  (*     replace ndom_src with ndom_tgt; et. *)
+  (*     unfold ndom_src, ndom_tgt. fold sk_src. rewrite SKEQ. clear -SIM. clearbody sk_tgt. *)
+  (*     rewrite !List.map_map. rewrite !ModSemFacts.fun_fst_trans_r. *)
+  (*     revert mds_tgt SIM. induction mds_src; i.  *)
+  (*     { inv SIM. destruct mds_tgt; clarify. } *)
+  (*     destruct mds_tgt; inv SIM. ss. unfold ModSem.add_fnsems. rewrite !map_app. *)
+  (*     rewrite !List.map_map.  *)
+  (*     rewrite !ModSemFacts.fun_fst_trans_l. *)
+  (*     rewrite !ModSemFacts.fun_fst_trans_r. f_equal; et. *)
+  (*     inv H3. clear -sim_fnsems. *)
+  (*     set (ModSem.fnsems _) as fl1. set (ModSem.fnsems _) as fl2.  *)
+  (*     fold fl1 in sim_fnsems. fold fl2 in sim_fnsems. *)
+  (*     clearbody fl1 fl2. revert fl2 sim_fnsems. *)
+  (*     induction fl1; i; destruct fl2; inv sim_fnsems; ss. *)
+  (*     f_equal; et. inv H3. destruct a0, p. ss. } *)
+  (*   ss. rewrite SKEQ. *)
+  (*   red in SIM. inv w. rename H0 into MSWFTGT. red in MSWFTGT. ss. fold sk_tgt in MSWFTGT.  *)
+  (*   clearbody sk_tgt. clear -SIM PR MSWFTGT. *)
+  (*   revert mds_tgt SIM ctx MSWFTGT x0 PR. *)
+  (*   induction mds_src; i. *)
+  (*   { destruct mds_tgt; inv SIM. ss. } *)
+  (*   destruct mds_tgt; inv SIM. ss. *)
+  (*   eapply ModSemFacts.add_assoc. { instantiate (1:= true). et. } *)
+  (*   eapply ModSemFacts.add_assoc_rev in PR. 2:{ instantiate (1:= true). et. } *)
+  (*   change (ModSem.add (Mod.get_modsem ctx (Sk.canon sk_tgt)) (Mod.get_modsem a (Sk.canon sk_tgt))) *)
+  (*     with (Mod.get_modsem (Mod.add ctx a) (Sk.canon sk_tgt)). *)
+  (*   eapply IHmds_src. { et. } *)
+  (*   { clear -MSWFTGT H3. inv MSWFTGT. econs; ss. *)
+  (*     unfold ModSem.add_fnsems in *; rewrite ! map_app in *. ss. *)
+  (*     unfold ModSem.add_fnsems in *; rewrite ! map_app in *. rewrite app_assoc in wf_fnsems. *)
+  (*     rewrite !List.map_map in *. *)
+  (*     rewrite ModSemFacts.fun_fst_trans_l_l. *)
+  (*     rewrite ModSemFacts.fun_fst_trans_l_r. *)
+  (*     rewrite ModSemFacts.fun_fst_trans_r. *)
+  (*     rewrite ModSemFacts.fun_fst_trans_l in wf_fnsems. *)
+  (*     rewrite ModSemFacts.fun_fst_trans_r_l in wf_fnsems. *)
+  (*     rewrite ModSemFacts.fun_fst_trans_r_r in wf_fnsems. *)
+  (*     set (List.map _ (ModSem.fnsems (Mod.get_modsem a _))) as anamedom. *)
+  (*     set (List.map _ (ModSem.fnsems (Mod.get_modsem t _))) as tnamedom in wf_fnsems. *)
+  (*     replace anamedom with tnamedom; et. *)
+  (*     unfold tnamedom, anamedom. inv H3. clear -sim_fnsems. *)
+  (*     induction sim_fnsems; auto. *)
+  (*     ss. f_equal; ss. inv H0. destruct x, y. ss. } *)
+  (*   ss.  *)
+  (*   eapply ModSemFacts.add_comm. { instantiate (1:= true). et. } *)
+  (*   { clear -MSWFTGT H3. inv MSWFTGT. econs; ss. *)
+  (*     unfold ModSem.add_fnsems in *; rewrite ! map_app in *. ss. *)
+  (*     unfold ModSem.add_fnsems in *; rewrite ! map_app in *. rewrite app_assoc in wf_fnsems. *)
+  (*     rewrite !List.map_map in *. *)
+  (*     rewrite ModSemFacts.fun_fst_trans_l_l. *)
+  (*     rewrite ModSemFacts.fun_fst_trans_l_r. *)
+  (*     rewrite ModSemFacts.fun_fst_trans_r. *)
+  (*     rewrite ModSemFacts.fun_fst_trans_l in wf_fnsems. *)
+  (*     rewrite ModSemFacts.fun_fst_trans_r_l in wf_fnsems. *)
+  (*     rewrite ModSemFacts.fun_fst_trans_r_r in wf_fnsems. *)
+  (*     set (List.map _ (ModSem.fnsems (Mod.get_modsem a _))) as anamedom. *)
+  (*     set (List.map _ (ModSem.fnsems (Mod.get_modsem t _))) as tnamedom in wf_fnsems. *)
+  (*     replace anamedom with tnamedom; et. *)
+  (*     unfold tnamedom, anamedom. inv H3. clear -sim_fnsems. *)
+  (*     induction sim_fnsems; auto. *)
+  (*     ss. f_equal; ss. inv H0. destruct x, y. ss. } *)
+  (*   eapply ModSemFacts.add_comm in PR; cycle 1. { instantiate (1:= true). et. } *)
+  (*   { clear -MSWFTGT H3. inv MSWFTGT. econs; ss. *)
+  (*     unfold ModSem.add_fnsems in *; rewrite ! map_app in *. ss. *)
+  (*     unfold ModSem.add_fnsems in *; rewrite ! map_app in *. rewrite app_assoc in wf_fnsems. *)
+  (*     rewrite !List.map_map in *. *)
+  (*     rewrite !ModSemFacts.fun_fst_trans_l in *. *)
+  (*     rewrite !ModSemFacts.fun_fst_trans_r_l in *. *)
+  (*     rewrite !ModSemFacts.fun_fst_trans_r_r in *. *)
+  (*     apply nodup_comm. et. } *)
+  (*   eapply ModSemFacts.add_assoc. { instantiate (1:= true). et. } *)
+  (*   eapply ModSemFacts.add_assoc_rev in PR. 2:{ instantiate (1:= true). et. } *)
+  (*   eapply adequacy_modsem; cycle 1; et. apply sim_ctx. et. *)
+  (* Qed. *)
+  Admitted.
 
-    ii.
-    apply sim_ctx_mod with (ctx:=ctx) in SIM.
-
-    pose (Mod.add md_src ctx) as mds.
-    pose (Mod.add md_tgt ctx) as mdt.
-    fold mds. fold mdt in PR.
-    apply adequacy_mod with (md_src := mds) in PR; et.
+  Corollary adequacy_local_strong md_src md_tgt
+      (SIM: ModPair.sim md_src md_tgt)
+    :
+      <<CR: (refines_strong md_tgt md_src)>>
+  .
+  Proof.
+    red. red. red. i.
+    replace md_src with (Mod.add_list [md_src]) by et.
+    replace md_tgt with (Mod.add_list [md_tgt]) in PR by et.
+    eapply adequacy_local_strong_l; et. i. inv SIM. econs; ss; et.
+    i. econs; et. eapply sim_modsem; et. inv SKINCL. ss.
   Qed.
+
+  (* Lemma sim_ctx_mod *)
+  (*   ctx md1 md2 *)
+  (*   (SIM: ModPair.sim md1 md2) *)
+
+  (* : *)
+  (*   ModPair.sim (Mod.add md1 ctx) (Mod.add md2 ctx) *)
+  (* . *)
+  (* Proof. *)
+  (*   inv SIM. *)
+  (*   econs; et. *)
+  (*   (* - i. ss. hexploit (sim_modsem sk); et. *) *)
+  (*   - i. ss. hexploit (sim_modsem sk); et. *)
+
+  (*     2: { ii. des. apply sim_ctx; et. } *)
+  (*     unfold Sk.incl, Sk.add in *. i. ss. *)
+  (*     apply SKINCL. *)
+  (*     rewrite in_app_iff. et. *)
+  (*   - r. ss. unfold Sk.add. ss. *)
+  (*     rewrite sim_sk. et. *)
+  (* Qed. *)
+
+  (* Lemma adequacy_mod *)
+  (*         md_src md_tgt *)
+  (*         (CONF: EMSConfig) *)
+  (*         (SIM: ModPair.sim md_src md_tgt) *)
+  (*   : *)
+  (*   <<REF: Beh.of_program (Mod.compile md_tgt) <1= Beh.of_program (Mod.compile md_src) >> *)
+  (*   . *)
+  (* Proof. *)
+  (*   ii. unfold Mod.compile in *. *)
+  (*   destruct (classic (ModSem.wf (Mod.enclose (md_src)) /\ Sk.wf (Mod.sk md_src))). *)
+  (*   2: { eapply ModSem.initial_itr_not_wf. ss. } *)
+  (*   ss. des.  *)
+  (*   pose (sk_tgt := (Mod.sk (md_tgt))). *)
+  (*   pose (sk_src := (Mod.sk (md_src))). *)
+  (*   assert (SKEQ: sk_src = sk_tgt). *)
+  (*   { unfold sk_tgt, sk_src. inv SIM. et. } *)
+  (*   unfold Mod.enclose in *. fold sk_src in H. inv H. *)
+  (*   inv SIM. hexploit (sim_modsem (Sk.canon sk_tgt)). *)
+  (*   { etrans; [|eapply Sk.sort_incl]. ss. } *)
+  (*   { ss. rewrite sim_sk in H0. *)
+  (*     clear - H0. *)
+  (*     unfold Sk.wf in *. ss. *)
+  (*     eapply Permutation.Permutation_NoDup; [|et]. *)
+  (*     eapply Permutation.Permutation_map. *)
+  (*     eapply Sk.SkSort.sort_permutation. } *)
+  (*   i. des. *)
+  (*   inv H. ss. *)
+
+  (*   assert (WFTGT: Mod.wf md_tgt). *)
+  (*   { rr. unfold Mod.enclose. ss. fold sk_tgt.  *)
+  (*     rewrite SKEQ in *. split; auto. *)
+  (*     2: { rewrite <-SKEQ. unfold sk_src. et. } *)
+  (*     econs. *)
+  (*     match goal with *)
+  (*       | H: NoDup ?l0 |- NoDup ?l1 => replace l1 with l0 *)
+  (*     end; auto. *)
+  (*     eapply Forall2_eq. eapply Forall2_apply_Forall2; et. *)
+  (*     i. destruct a, b. inv H. ss. *)
+  (*   } *)
+
+  (*   eapply adequacy_local_aux in PR; et. *)
+  (*   - i. esplits. *)
+  (*     pose (ms_src := Mod.get_modsem md_src (Sk.sort (Mod.sk md_src))). *)
+  (*     pose (ms_tgt := Mod.get_modsem md_tgt (Sk.sort (Mod.sk md_tgt))). *)
+  (*     fold ms_src ms_tgt. *)
+  (*     rewrite <- SKEQ in sim_fnsems at 1. *)
+  (*     unfold sk_src, sk_tgt in sim_fnsems. *)
+  (*     fold ms_src ms_tgt in sim_fnsems. *)
+  (*     hexploit sim_fnsems. i. *)
+
+  (*     destruct (alist_find fn (ModSem.fnsems ms_src)) eqn:SRC; destruct (alist_find fn (ModSem.fnsems ms_tgt)) eqn:TGT; et. *)
+  (*     2: { *)
+  (*       right. *)
+  (*       eapply alist_find_some in SRC. *)
+  (*       rewrite <- sim_sk in sim_fnsems. *)
+  (*       (* eapply alist_find_none in TGT. *) *)
+  (*       eapply Forall2_In_l with (a:= (fn, i)) in sim_fnsems; et. *)
+  (*       inv sim_fnsems. inv H1. *)
+  (*       inv H3. inv H1. *)
+  (*       destruct x. ss. clarify. *)
+  (*       apply alist_find_none with (v:=i0) in TGT. clarify.  *)
+  (*     } *)
+  (*     right. esplits; et. *)
+
+  (*     hexploit SRC. hexploit TGT. i. *)
+  (*     apply alist_find_some in H1, H2. *)
+
+  (*     rewrite <- sim_sk in sim_fnsems. *)
+
+  (*     eapply Forall2_In_l with (a:=(fn, i)) in sim_fnsems; et. *)
+  (*     eapply Forall2_In_r with (b:=(fn, i0)) in H; et. *)
+  (*     inv sim_fnsems. inv H. *)
+  (*     destruct x, x1. *)
+  (*     inv H3. inv H5. inv H3. ss. *)
+  (*     inv H4. inv H7. inv H4. ss. clarify. *)
+  (*     unfold "@@2" in H5, H6. ss. *)
+  (*     (* apply NoDup_map_inv in wf_fnsems. *) *)
+  (*     unfold sk_src in wf_fnsems. *)
+  (*     fold ms_src in wf_fnsems. *)
+  (*     rewrite <- sim_sk in H3. *)
+  (*     eapply alist_find_some_iff  with (k:=s) (v:=i2) in wf_fnsems; et. *)
+  (*     rewrite SRC in wf_fnsems. clarify. apply H5. *)
+  (*   (* - inv sim_initial. econs. econs. *)
+  (*     2: { fold sk_src sk_tgt. rewrite SKEQ. apply H. } *)
+  (*     instantiate (1:= x). refl. *) *)
+
+  (*   Qed. *)
+
+
+  (* Theorem adequacy_local_strong md_src md_tgt *)
+  (*         (SIM: ModPair.sim md_src md_tgt) *)
+  (*   : *)
+  (*   <<CR: (refines_strong md_tgt md_src)>> *)
+  (* . *)
+  (* Proof. *)
+
+  (*   ii. *)
+  (*   apply sim_ctx_mod with (ctx:=ctx) in SIM. *)
+
+  (*   pose (Mod.add md_src ctx) as mds. *)
+  (*   pose (Mod.add md_tgt ctx) as mdt. *)
+  (*   fold mds. fold mdt in PR. *)
+  (*   apply adequacy_mod with (md_src := mds) in PR; et. *)
+  (* Qed. *)
 
   Context {CONF: EMSConfig}.
 
-  Theorem adequacy_local md_src md_tgt
+  Corollary adequacy_local md_src md_tgt
           (SIM: ModPair.sim md_src md_tgt)
     :
       <<CR: (refines md_tgt md_src)>>
@@ -163,63 +317,63 @@ Section ADEQUACY.
     eapply adequacy_local_strong; et.
   Qed.
 
-  Corollary adequacy_local_list_strong
-            mds_src mds_tgt
-            (FORALL: List.Forall2 ModPair.sim mds_src mds_tgt)
-    :
-      <<CR: refines_strong (Mod.add_list mds_tgt) (Mod.add_list mds_src)>>
-  .
-  Proof.
-    (* apply adequacy_local_strong. *)
+  (* Corollary adequacy_local_list_strong *)
+  (*           mds_src mds_tgt *)
+  (*           (FORALL: List.Forall2 ModPair.sim mds_src mds_tgt) *)
+  (*   : *)
+  (*     <<CR: refines_strong (Mod.add_list mds_tgt) (Mod.add_list mds_src)>> *)
+  (* . *)
+  (* Proof. *)
+  (*   (* apply adequacy_local_strong. *) *)
 
-  (* Admitted. *)
+  (* (* Admitted. *) *)
 
 
-    r. induction FORALL; ss.
-    { ii. auto. }
+  (*   r. induction FORALL; ss. *)
+  (*   { ii. auto. } *)
 
-      destruct l eqn: L, l' eqn: L'.
-      - apply adequacy_local_strong; et.
-      - etrans.
-        + instantiate (1:= Mod.add x (Mod.add_list [])). apply refines_strong_add.
-          * apply adequacy_local_strong. apply H.
-          * apply IHFORALL.
-        + s. ii.
-          pose proof ModFacts.add_comm as COMM. 
-          pose proof ModFacts.add_assoc_rev as ASSOC'.
-          apply COMM. apply COMM in PR. apply ASSOC' in PR. apply ModFacts.add_empty_r in PR. et.
-      - etrans.
-        + apply adequacy_local_strong. apply H.
-        + etrans.
-          * instantiate (1:= Mod.add x (Mod.add_list [])). s. ii.
-            pose proof ModFacts.add_comm as COMM. 
-            pose proof ModFacts.add_assoc as ASSOC.
-            apply COMM. apply COMM in PR. apply ASSOC. apply ModFacts.add_empty_rev_r. apply PR.
-          * apply refines_strong_add; et. apply adequacy_local_strong.
-            econs; et. ii. rr. apply ModSemPair.self_sim.
-      - apply refines_strong_add; et. apply adequacy_local_strong. apply H.
-    Qed.             
+  (*     destruct l eqn: L, l' eqn: L'. *)
+  (*     - apply adequacy_local_strong; et. *)
+  (*     - etrans. *)
+  (*       + instantiate (1:= Mod.add x (Mod.add_list [])). apply refines_strong_add. *)
+  (*         * apply adequacy_local_strong. apply H. *)
+  (*         * apply IHFORALL. *)
+  (*       + s. ii. *)
+  (*         pose proof ModFacts.add_comm as COMM.  *)
+  (*         pose proof ModFacts.add_assoc_rev as ASSOC'. *)
+  (*         apply COMM. apply COMM in PR. apply ASSOC' in PR. apply ModFacts.add_empty_r in PR. et. *)
+  (*     - etrans. *)
+  (*       + apply adequacy_local_strong. apply H. *)
+  (*       + etrans. *)
+  (*         * instantiate (1:= Mod.add x (Mod.add_list [])). s. ii. *)
+  (*           pose proof ModFacts.add_comm as COMM.  *)
+  (*           pose proof ModFacts.add_assoc as ASSOC. *)
+  (*           apply COMM. apply COMM in PR. apply ASSOC. apply ModFacts.add_empty_rev_r. apply PR. *)
+  (*         * apply refines_strong_add; et. apply adequacy_local_strong. *)
+  (*           econs; et. ii. rr. apply ModSemPair.self_sim. *)
+  (*     - apply refines_strong_add; et. apply adequacy_local_strong. apply H. *)
+  (*   Qed.              *)
           
 
-  Theorem adequacy_local2 md_src md_tgt
-          (SIM: ModPair.sim md_src md_tgt)
-    :
-      <<CR: (refines2 [md_tgt] [md_src])>>
-  .
-  Proof.
-    eapply refines_strong_refines.
-    eapply adequacy_local_list_strong. econs; ss.
-  Qed.
+  (* Theorem adequacy_local2 md_src md_tgt *)
+  (*         (SIM: ModPair.sim md_src md_tgt) *)
+  (*   : *)
+  (*     <<CR: (refines2 [md_tgt] [md_src])>> *)
+  (* . *)
+  (* Proof. *)
+  (*   eapply refines_strong_refines. *)
+  (*   eapply adequacy_local_list_strong. econs; ss. *)
+  (* Qed. *)
 
-  Corollary adequacy_local_list
-            mds_src mds_tgt
-            (FORALL: List.Forall2 ModPair.sim mds_src mds_tgt)
-    :
-      <<CR: refines (Mod.add_list mds_tgt) (Mod.add_list mds_src)>>
-  .
-  Proof.
-    eapply refines_strong_refines.
-    eapply adequacy_local_list_strong; et.
-  Qed.
+  (* Corollary adequacy_local_list *)
+  (*           mds_src mds_tgt *)
+  (*           (FORALL: List.Forall2 ModPair.sim mds_src mds_tgt) *)
+  (*   : *)
+  (*     <<CR: refines (Mod.add_list mds_tgt) (Mod.add_list mds_src)>> *)
+  (* . *)
+  (* Proof. *)
+  (*   eapply refines_strong_refines. *)
+  (*   eapply adequacy_local_list_strong; et. *)
+  (* Qed. *)
 
 End ADEQUACY.
